using nat instead of access_size allows completing
StateMachineMMIO.compile_ext_call_correct, but the
files that need to satisfy the new assumptions of
StateMachineSemantics still don't work

investigations/bedrock2/LibBase/MMIOLabels.v
@@ -1,7 +1,8 @@
 (* names for the MMIO load/store events to record in the I/O trace *)
 
 Require Import Coq.Strings.String. Local Open Scope string_scope.
-Require Import bedrock2.Syntax.
+Require Import Coq.Numbers.DecimalString.
+Require Import Coq.Numbers.DecimalNat.
 
 Definition READ_PREFIX := "MMIOREAD".
 Definition READ8 := READ_PREFIX ++ "8".
@@ -15,37 +16,37 @@ Definition WRITE16 := WRITE_PREFIX ++ "16".
 Definition WRITE32 := WRITE_PREFIX ++ "32".
 Definition WRITE64 := WRITE_PREFIX ++ "64".
 
-Require Import coqutil.Word.Interface.
-Require Import Coq.Numbers.DecimalString.
-Require Import Coq.ZArith.ZArith.
+Definition natToStr(n: nat): string := DecimalString.NilEmpty.string_of_uint (Nat.to_uint n).
 
-Definition ZToStr(n: Z): string := DecimalString.NilZero.string_of_int (Z.to_int n).
+Definition access_size_to_MMIO_read(sz: nat): string :=
+  READ_PREFIX ++ natToStr (sz * 8).
 
-Definition access_size_to_MMIO_suffix(width: Z)(sz: access_size): string :=
-  match sz with
-  | access_size.one => "8"
-  | access_size.two => "16"
-  | access_size.four => "32"
-  | access_size.word => ZToStr width
-  end.
+Definition access_size_to_MMIO_write(sz: nat): string :=
+  WRITE_PREFIX ++ natToStr (sz * 8).
 
-(* We pass an unnecessary `word` instance to the following definitions just to make
-   `width` inferrable, later we might make a typeclass for just `width` and then we
-   can remove the `word`. *)
-#[export] Hint Mode word.word - : typeclass_instances.
+Lemma string_of_uint_inj: forall n m, NilEmpty.string_of_uint n = NilEmpty.string_of_uint m -> n = m.
+Proof.
+  intros. apply (f_equal NilEmpty.uint_of_string) in H.
+  do 2 rewrite NilEmpty.usu in H.
+  inversion H.
+  reflexivity.
+Qed.
 
-Definition access_size_to_MMIO_read{width}{word: word.word width}(sz: access_size): string :=
-  READ_PREFIX ++ access_size_to_MMIO_suffix width sz.
+Lemma natToStr_inj: forall n m, natToStr n = natToStr m -> n = m.
+Proof.
+  unfold natToStr. intros.
+  apply string_of_uint_inj in H.
+  apply Unsigned.to_uint_inj in H.
+  exact H.
+Qed.
 
-Definition access_size_to_MMIO_write{width}{word: word.word width}(sz: access_size): string :=
-  WRITE_PREFIX ++ access_size_to_MMIO_suffix width sz.
-
-Lemma access_size_to_MMIO_read_inj{width}{word: word.word width}: forall sz1 sz2,
+Lemma access_size_to_MMIO_read_inj: forall sz1 sz2,
     access_size_to_MMIO_read sz1 = access_size_to_MMIO_read sz2 ->
     sz1 = sz2.
 Proof.
-  destruct sz1; destruct sz2; cbn; try congruence; intros.
-  3: {
-    inversion H.
-    (* doesn't hold!! *)
-Admitted.
+  unfold access_size_to_MMIO_read.
+  intros. inversion H.
+  apply natToStr_inj in H1.
+  eapply PeanoNat.Nat.mul_cancel_r. 2: eassumption.
+  discriminate.
+Qed.
