investigations/bedrock2/StateMachineSemantics.v
@@ -18,8 +18,8 @@ Module parameters.
     { state : Type;
       register : Type;
       is_initial_state : state -> Prop;
-      read_step : access_size -> state -> register -> word -> state -> Prop;
-      write_step : access_size -> state -> register -> word -> state -> Prop;
+      read_step : nat(*how many bytes (1,2,4,8)*) -> state -> register -> word -> state -> Prop;
+      write_step : nat(*how many bytes (1,2,4,8)*) -> state -> register -> word -> state -> Prop;
       reg_addr : register -> word;
       isMMIOAddr : word -> Prop;
     }.
@@ -27,24 +27,32 @@ Module parameters.
 
   Class ok {width word mem} (p : parameters width word mem) :=
     { width_ok : width = 32 \/ width = 64;
-      word_ok : word.ok word; (* for impl of mem below *)
-      mem_ok : Interface.map.ok mem; (* for impl of mem below *)
+      word_ok :> word.ok word; (* for impl of mem below *)
+      mem_ok :> Interface.map.ok mem; (* for impl of mem below *)
       reg_addr_unique : forall r1 r2, reg_addr r1 = reg_addr r2 -> r1 = r2;
-      read_step_isMMIOAddr : forall sz s a v s',
-          read_step sz s a v s' ->
-          isMMIOAddr (reg_addr a);
-      write_step_isMMIOAddr : forall sz s a v s',
-          write_step sz s a v s' ->
-          isMMIOAddr (reg_addr a);
-      read_step_is_aligned : forall sz s a v s',
-          read_step sz s a v s' ->
-          word.unsigned (reg_addr a) mod (Z.of_nat (Memory.bytes_per (width := width) sz)) = 0;
-      write_step_is_aligned : forall sz s a v s',
-          write_step sz s a v s' ->
-          word.unsigned (reg_addr a) mod (Z.of_nat (Memory.bytes_per (width := width) sz)) = 0;
-      read_step_bounded : forall sz s a v s',
-          read_step sz s a v s' ->
-          word.unsigned v < 2 ^ (8 * Z.of_nat (Memory.bytes_per (width := width) sz));
+      read_step_isMMIOAddr : forall sz s r v s',
+          read_step sz s r v s' -> forall a: word,
+            word.unsigned (reg_addr r) <= word.unsigned a < word.unsigned (reg_addr r) + Z.of_nat sz ->
+            isMMIOAddr a;
+      write_step_isMMIOAddr : forall sz s r v s',
+          write_step sz s r v s' -> forall a: word,
+            word.unsigned (reg_addr r) <= word.unsigned a < word.unsigned (reg_addr r) + Z.of_nat sz ->
+            isMMIOAddr a;
+      read_step_is_aligned : forall sz s r v s',
+          read_step sz s r v s' ->
+          word.unsigned (reg_addr r) mod (Z.of_nat sz) = 0;
+      write_step_is_aligned : forall sz s r v s',
+          write_step sz s r v s' ->
+          word.unsigned (reg_addr r) mod (Z.of_nat sz) = 0;
+      read_step_size_valid : forall sz s r v s',
+          read_step sz s r v s' ->
+          List.In sz [1; 2; 4]%nat;
+      write_step_size_valid : forall sz s r v s',
+          write_step sz s r v s' ->
+          List.In sz [1; 2; 4]%nat;
+      read_step_bounded : forall sz s r v s',
+          read_step sz s r v s' ->
+          word.unsigned v < 2 ^ (Z.of_nat sz * 8);
       (* Note: It would be nice if we could allow too big writes and just ignore the upper
          bytes, but then we run into a specification issue: bedrock2 semantics of external
          calls (exec.interact) puts the whole unmodified word into the trace, and we want
@@ -52,9 +60,9 @@ Module parameters.
          introducing a notion of trace equivalence), but riscv-coq cannot put the upper
          ignored bits into the trace, because riscv.Spec.ExecuteI does not pass them
          to nonmem_store *)
-      write_step_bounded : forall sz s a v s',
-          write_step sz s a v s' ->
-          word.unsigned v < 2 ^ (Z.of_nat (Memory.bytes_per (width := width) sz) * 8);
+      write_step_bounded : forall sz s r v s',
+          write_step sz s r v s' ->
+          word.unsigned v < 2 ^ (Z.of_nat sz * 8);
     }.
 End parameters.
 Notation parameters := parameters.parameters.
@@ -170,15 +178,28 @@ Section WithParameters.
   Proof.
     split; cbv [env locals semantics_parameters]; try exact _.
     { exact width_ok. }
-    { exact word_ok. }
-    { exact mem_ok. }
     { exact (SortedListString.ok _). }
     { exact (SortedListString.ok _). }
-  Defined.
+  Qed.
 
   (* COPY-PASTE this *)
-  Add Ring wring : (Properties.word.ring_theory (word := Semantics.word))
+  Add Ring wring : (Properties.word.ring_theory (word := word))
         (preprocess [autorewrite with rew_word_morphism],
-         morphism (Properties.word.ring_morph (word := Semantics.word)),
+         morphism (Properties.word.ring_morph (word := word)),
          constants [Properties.word_cst]).
+
+  Lemma read_step_isMMIOAddr0: forall sz s a v s',
+      read_step sz s a v s' -> isMMIOAddr (reg_addr a).
+  Proof.
+    intros. eapply read_step_isMMIOAddr. 1: exact H.
+    apply read_step_size_valid in H. simpl in H. Lia.lia.
+  Qed.
+
+  Lemma write_step_isMMIOAddr0: forall sz s a v s',
+      write_step sz s a v s' -> isMMIOAddr (reg_addr a).
+  Proof.
+    intros. eapply write_step_isMMIOAddr. 1: exact H.
+    apply write_step_size_valid in H. simpl in H. Lia.lia.
+  Qed.
+
 End WithParameters.
